Iris/Iris/Algebra/OFE.lean
@@ -155,27 +155,27 @@ class Contractive [OFE α] [OFE β] (f : α → β) where
 
 attribute [aesop_contractive safe apply] Contractive.distLater_dist
 
-@[simp, rocq_alias contractive_0] theorem Contractive.zero [OFE α] [OFE β] (f : α → β)
+@[simp, aesop_contractive safe apply, rocq_alias contractive_0] theorem Contractive.zero [OFE α] [OFE β] (f : α → β)
     [Contractive f] {x y} : f x ≡{0}≡ f y :=
   Contractive.distLater_dist distLater_zero
 
-@[rocq_alias contractive_S]
+@[aesop_contractive safe apply, rocq_alias contractive_S]
 theorem Contractive.succ [OFE α] [OFE β] (f : α → β) [Contractive f] {n x y}
     (h : x ≡{n}≡ y) : f x ≡{n.succ}≡ f y :=
   Contractive.distLater_dist (distLater_succ.2 h)
 
 /-- A contractive function is non-expansive. -/
-@[rocq_alias contractive_ne]
+@[aesop_contractive safe apply, rocq_alias contractive_ne]
 instance ne_of_contractive [OFE α] [OFE β] (f : α → β) [Contractive f] : NonExpansive f where
   ne := fun _ _ _ h => Contractive.distLater_dist (Dist.distLater h)
 
 /-- A contractive function preserves equivalence. -/
-@[rocq_alias contractive_proper]
+@[aesop_contractive safe apply, rocq_alias contractive_proper]
 theorem Contractive.eqv [OFE α] [OFE β] (f : α → β) [Contractive f] ⦃x y : α⦄ (h : x ≡ y) :
     f x ≡ f y := NonExpansive.eqv h
 
 /-- Constant functions are contractive. -/
-@[rocq_alias const_contractive]
+@[aesop_contractive safe apply, rocq_alias const_contractive]
 instance [OFE α] [OFE β] {x : β} : Contractive (fun _ : α => x) where
   distLater_dist := fun _ => Dist.rfl
 
